CollapsingTowers/TwoLevelMut/OperationalSemantics/Defs.lean
@@ -1,3 +1,4 @@
 import CollapsingTowers.TwoLevelMut.OperationalSemantics.Value
+import CollapsingTowers.TwoLevelMut.OperationalSemantics.Store
 import CollapsingTowers.TwoLevelMut.OperationalSemantics.EvalCtx
 import CollapsingTowers.TwoLevelMut.OperationalSemantics.SmallStep
