CollapsingTowers/TwoLevelMut/SyntacticSoundness/Defs.lean
@@ -2,4 +2,5 @@ import CollapsingTowers.TwoLevelMut.SyntacticSoundness.PresvSubst
 import CollapsingTowers.TwoLevelMut.SyntacticSoundness.PresvMaping
 import CollapsingTowers.TwoLevelMut.SyntacticSoundness.PresvCtx
 import CollapsingTowers.TwoLevelMut.SyntacticSoundness.PresvPure
+import CollapsingTowers.TwoLevelMut.SyntacticSoundness.PresvMut
 import CollapsingTowers.TwoLevelMut.SyntacticSoundness.Preservation
