CollapsingTowers/TwoLevelMut/SyntacticSoundness/Preservation.lean
@@ -1,4 +1,5 @@
 import CollapsingTowers.TwoLevelMut.SyntacticSoundness.PresvPure
+import CollapsingTowers.TwoLevelMut.SyntacticSoundness.PresvMut
 
 theorem preservation.strengthened :
   ∀ Γ σ₀ σ₁ e₀ e₁ τ φ₀,
@@ -19,15 +20,23 @@ theorem preservation.strengthened :
       cases φ <;> simp at Hφ
       constructor
       . apply Hok₀
-      . exists ⊥
-        exact ⟨typing_reification.pure _ _ _ _ Hτ, rfl⟩
+      . exists ⊥; exact ⟨typing_reification.pure _ _ _ _ Hτ, rfl⟩
     case reify Hτ =>
       have ⟨φ, Hτ, Hφ⟩ := preservation.pure _ _ _ _ _ _ _ HM Hlc Hhead Hτ
       constructor
       . apply Hok₀
-      . exists φ
-        exact ⟨typing_reification.reify _ _ _ _ _ Hτ, Hφ⟩
+      . exists φ; exact ⟨typing_reification.reify _ _ _ _ _ Hτ, Hφ⟩
   case mutable HM Hlc Hmut =>
-    admit
+    cases Hτ
+    case pure Hτ =>
+      have ⟨Hok₁, Hτ⟩ := preservation.mutable _ _ _ _ _ _ _ _ HM Hlc Hmut Hok₀ Hτ
+      constructor
+      . apply Hok₁
+      . exists ⊥; exact ⟨typing_reification.pure _ _ _ _ Hτ, rfl⟩
+    case reify Hτ =>
+      have ⟨Hok₁, Hτ⟩ := preservation.mutable _ _ _ _ _ _ _ _ HM Hlc Hmut Hok₀ Hτ
+      constructor
+      . apply Hok₁
+      . exists φ₀; exact ⟨typing_reification.reify _ _ _ _ _ Hτ, (by simp)⟩
   case reflect P E e HP HE Hlc =>
     admit
