CollapsingTowers/TwoLevelMut/SyntacticSoundness/PresvMut.lean
@@ -1,0 +1,144 @@
+import CollapsingTowers.TwoLevelMut.SyntacticSoundness.PresvCtx
+
+theorem preservation.mutable.head :
+  ∀ σ₀ σ₁ Γ e₀ e₁ τ φ,
+    head_mutable ⟨σ₀, e₀⟩ ⟨σ₁, e₁⟩ →
+    ok σ₀ →
+    typing σ₀ Γ 𝟙 e₀ τ φ →
+    ok σ₁ ∧
+    typing σ₁ Γ 𝟙 e₁ τ φ :=
+  by
+  intros σ₀ σ₁ Γ e₀ e₁ τ φ Hmut Hok₀ Hτ
+  cases Hmut
+  case alloc₁ v Hvalue =>
+    cases Hτ
+    case alloc₁ Hτe =>
+    cases Hvalue <;> try contradiction
+    case lit n =>
+      constructor
+      . apply ok.cons _ _ Hok₀
+      . cases Hτe; apply typing.loc; simp
+  case load₁ l Hbinds =>
+    cases Hτ
+    case load₁ Hτe =>
+    constructor
+    . apply Hok₀
+    . have ⟨n, HEq⟩ := ok.binds _ _ _ Hok₀ Hbinds
+      rw [← HEq]
+      cases Hτe; apply typing.lit
+  case store₁ l v Hvalue Hpatch =>
+    cases Hτ
+    case store₁ Hτl Hτr =>
+    cases Hvalue <;> try contradiction
+    case lit n =>
+      constructor
+      . apply ok.patch _ _ _ _ Hpatch Hok₀
+      . cases Hτl; cases Hτr; apply typing.unit
+
+theorem preservation.mutable :
+  ∀ σ₀ σ₁ Γ M e₀ e₁ τ φ,
+    ctx𝕄 Γ.length M →
+    lc e₀ →
+    head_mutable ⟨σ₀, e₀⟩ ⟨σ₁, e₁⟩ →
+    ok σ₀ →
+    typing σ₀ Γ 𝟙 M⟦e₀⟧ τ φ →
+    ok σ₁ ∧
+    typing σ₁ Γ 𝟙 M⟦e₁⟧ τ φ :=
+  by
+  intros σ₀ σ₁ Γ M e₀ e₁ τ φ HM Hlc Hmut Hok₀ Hτ
+  generalize HEqlvl : Γ.length = lvl
+  rw [HEqlvl] at HM
+  have HLe := head_mutable.store_grow _ _ _ _ Hmut
+  induction HM generalizing Γ τ φ
+  case hole => apply preservation.mutable.head _ _ _ _ _ _ _ Hmut Hok₀ Hτ
+  case cons𝔹 B M HB HM IH =>
+    have ⟨τ𝕖, φ₁, φ₂, HEqφ, Hτ, IHτB⟩ := preservation.under_ctx𝔹 _ _ _ _ _ _ HB Hτ
+    rw [HEqφ]
+    have ⟨Hok₁, Hτ⟩ := IH _ _ _ Hτ HEqlvl
+    have Hτ := IHτB _ ⦰ _ _ HLe Hτ
+    constructor
+    . apply Hok₁
+    . apply Hτ
+  case consℝ R M HR HM IH =>
+    rw [← HEqlvl] at HR IH
+    have Hlc : lc M⟦e₀⟧ := lc.under_ctx𝕄 _ _ _ _ HM Hlc
+    have Hfv : fv M⟦e₁⟧ ⊆ fv M⟦e₀⟧ := fv.under_ctx𝕄 _ _ _ _ HM (head_mutable.fv_shrink _ _ _ _ Hok₀ Hmut)
+    cases HR
+    case lam𝕔 =>
+      cases Hτ
+      case lam𝕔 Hwbt HX Hclosed =>
+        rw [identity.opening_closing _ _ _ Hlc] at HX
+        cases HX
+        case pure HX =>
+          have ⟨Hok₁, HX⟩ := IH (_ :: Γ) _ _ HX (by simp)
+          constructor
+          . apply Hok₁
+          . apply typing.lam𝕔
+            . apply typing_reification.pure
+              rw [identity.opening_closing _ _ _ (typing.regular _ _ _ _ _ _ HX)]
+              apply HX
+            . apply Hwbt
+            . rw [← closed.under_closing]
+              apply typing.closed_at_env _ _ _ _ _ _ HX
+        case reify HX =>
+          have ⟨Hok₁, HX⟩ := IH (_ :: Γ) _ _ HX (by simp)
+          constructor
+          . apply Hok₁
+          . apply typing.lam𝕔
+            . apply typing_reification.reify
+              rw [identity.opening_closing _ _ _ (typing.regular _ _ _ _ _ _ HX)]
+              apply HX
+            . apply Hwbt
+            . rw [← closed.under_closing]
+              apply typing.closed_at_env _ _ _ _ _ _ HX
+    case lets𝕔 =>
+      cases Hτ
+      case lets𝕔 Hwbt Hb HX Hclosed =>
+        rw [identity.opening_closing _ _ _ Hlc] at HX
+        cases HX
+        case pure HX =>
+          have ⟨Hok₁, HX⟩ := IH (_ :: Γ) _ _ HX (by simp)
+          constructor
+          . apply Hok₁
+          . apply typing.lets𝕔
+            . apply typing.weakening.store _ _ _ _ _ _ _ HLe Hb
+            . apply typing_reification.pure
+              rw [identity.opening_closing _ _ _ (typing.regular _ _ _ _ _ _ HX)]
+              apply HX
+            . apply Hwbt
+            . rw [← closed.under_closing]
+              apply typing.closed_at_env _ _ _ _ _ _ HX
+        case reify HX =>
+          have ⟨Hok₁, HX⟩ := IH (_ :: Γ) _ _ HX (by simp)
+          constructor
+          . apply Hok₁
+          . apply typing.lets𝕔
+            . apply typing.weakening.store _ _ _ _ _ _ _ HLe Hb
+            . apply typing_reification.reify
+              rw [identity.opening_closing _ _ _ (typing.regular _ _ _ _ _ _ HX)]
+              apply HX
+            . apply Hwbt
+            . rw [← closed.under_closing]
+              apply typing.closed_at_env _ _ _ _ _ _ HX
+    case run =>
+      cases Hτ
+      case run Hclosed HX =>
+        cases HX
+        case pure HX =>
+          have ⟨Hok₁, HX⟩ := IH _ _ _ HX rfl
+          constructor
+          . apply Hok₁
+          . apply typing.run
+            . apply typing_reification.pure _ _ _ _ HX
+            . rw [closed_iff_fv_empty] at Hclosed
+              simp [Hclosed] at Hfv
+              rw [closed_iff_fv_empty, Hfv]
+        case reify HX =>
+          have ⟨Hok₁, HX⟩ := IH _ _ _ HX rfl
+          constructor
+          . apply Hok₁
+          . apply typing.run
+            . apply typing_reification.reify _ _ _ _ _ HX
+            . rw [closed_iff_fv_empty] at Hclosed
+              simp [Hclosed] at Hfv
+              rw [closed_iff_fv_empty, Hfv]
